src/goose_lang/lib/typed_map/typed_map.v
@@ -1,0 +1,167 @@
+From iris.proofmode Require Import coq_tactics reduction.
+From Perennial.goose_lang Require Import notation proofmode typing.
+From Perennial.goose_lang.lib Require Import typed_mem.
+From Perennial.goose_lang.lib Require Import map.impl.
+From Perennial.goose_lang.lib Require map.map.
+Import uPred.
+
+From iris_string_ident Require Import ltac2_string_ident.
+
+Set Default Proof Using "Type".
+
+Class IntoVal {ext: ext_op} V :=
+  { to_val: V -> val;
+    IntoVal_def: V;
+  }.
+
+Class IntoValForType {ext V} (H: @IntoVal ext V) {ext_ty: ext_types ext} (t:ty) :=
+    { def_is_zero: to_val IntoVal_def = zero_val t;
+      (* TODO: this isn't necessary, but it seems reasonable *)
+      to_val_ty: forall v, val_ty (to_val v) t; }.
+
+Instance u64_IntoVal {ext: ext_op} : IntoVal u64 :=
+  {| to_val := λ (x: u64), LitV (LitInt x);
+     IntoVal_def := U64 0; |}.
+
+Instance u64_IntoVal_uint64T {ext} {ext_ty: ext_types ext} : IntoValForType u64_IntoVal uint64T.
+Proof.
+  constructor; auto.
+Qed.
+
+Module Map.
+  Definition t V {ext} `{@IntoVal ext V} := gmap u64 V.
+  Definition untype `{IntoVal V}:
+    t V -> gmap u64 val * val :=
+    fun m => (to_val <$> m, to_val IntoVal_def).
+End Map.
+
+Section heap.
+Context `{ffi_sem: ext_semantics} `{!ffi_interp ffi} `{!heapG Σ}.
+Context {ext_ty: ext_types ext}.
+
+Context `{!IntoVal V}.
+Context `{!IntoValForType IntoVal0 t}.
+
+Implicit Types (m: Map.t V) (k: u64) (v:V).
+
+Definition map_get m k : V * bool :=
+  let r := default IntoVal_def (m !! k) in
+  let ok := bool_decide (is_Some (m !! k)) in
+  (r, ok).
+
+Definition map_insert m k v : Map.t V :=
+  <[ k := v ]> m.
+
+Definition map_del m k : Map.t V :=
+  delete k m.
+
+Lemma map_get_true k v m :
+  map_get m k = (v, true) ->
+  m !! k = Some v.
+Proof.
+  rewrite /map_get.
+  destruct (m !! k); rewrite /=; congruence.
+Qed.
+
+Lemma map_get_false k v m :
+  map_get m k = (v, false) ->
+  m !! k = None ∧ v = IntoVal_def.
+Proof.
+  rewrite /map_get.
+  destruct (m !! k); rewrite /=.
+  - congruence.
+  - intuition congruence.
+Qed.
+
+Definition is_map (mref:loc) (m: Map.t V) :=
+  map.is_map mref (Map.untype m).
+
+Theorem is_map_untype mref m : is_map mref m -∗ map.is_map mref (Map.untype m).
+Proof.
+  auto.
+Qed.
+
+Theorem is_map_retype mref m : map.is_map mref (to_val <$> m, to_val IntoVal_def) -∗ is_map mref m.
+Proof.
+  auto.
+Qed.
+
+Ltac untype :=
+  rewrite /is_map /Map.untype.
+
+Theorem wp_NewMap stk E :
+  {{{ True }}}
+    NewMap t @ stk; E
+  {{{ mref, RET #mref;
+      is_map mref ∅ }}}.
+Proof using IntoValForType0.
+  iIntros (Φ) "_ HΦ".
+  wp_apply map.wp_NewMap.
+  iIntros (mref) "Hm".
+  iApply "HΦ".
+  iApply is_map_retype.
+  rewrite def_is_zero fmap_empty.
+  auto.
+Qed.
+
+Lemma map_get_fmap {m} {k} {vv: val} {ok: bool} :
+  map.map_get (Map.untype m) k = (vv, ok) ->
+  exists v, vv = to_val v ∧
+            map_get m k = (v, ok).
+Proof.
+  rewrite /map.map_get /map_get.
+  rewrite /Map.untype.
+  intros H; inversion H; subst; clear H.
+  destruct ((to_val <$> m) !! k) eqn:Hlookup; simpl; eauto.
+  - rewrite lookup_fmap in Hlookup.
+    apply fmap_Some in Hlookup as [x [Hlookup ->]].
+    rewrite Hlookup; eauto.
+  - eexists; intuition eauto.
+    rewrite lookup_fmap in Hlookup.
+    apply fmap_None in Hlookup.
+    rewrite Hlookup; auto.
+Qed.
+
+Theorem wp_MapGet stk E mref m k :
+  {{{ is_map mref m }}}
+    MapGet #mref #k @ stk; E
+  {{{ v ok, RET (to_val v, #ok);
+      ⌜map_get m k = (v, ok)⌝ ∗
+      is_map mref m }}}.
+Proof.
+  iIntros (Φ) "Hm HΦ".
+  iDestruct (is_map_untype with "Hm") as "Hm".
+  wp_apply (map.wp_MapGet with "Hm").
+  iIntros (vv ok) "(%Hmapget&Hm)".
+  apply map_get_fmap in Hmapget as [v [-> Hmapget]].
+  iApply "HΦ".
+  iSplit; [ auto | ].
+  iApply (is_map_retype with "Hm").
+Qed.
+
+Theorem map_insert_fmap m k v' :
+  map.map_insert (Map.untype m) k (to_val v') =
+  Map.untype (map_insert m k v').
+Proof.
+  untype.
+  rewrite /map.map_insert /map_insert.
+  rewrite fmap_insert //.
+Qed.
+
+Theorem wp_MapInsert stk E mref m k v' vv :
+  vv = to_val v' ->
+  {{{ is_map mref m }}}
+    MapInsert #mref #k vv @ stk; E
+  {{{ RET #(); is_map mref (map_insert m k v') }}}.
+Proof.
+  intros ->.
+  iIntros (Φ) "Hm HΦ".
+  iDestruct (is_map_untype with "Hm") as "Hm".
+  wp_apply (map.wp_MapInsert with "Hm").
+  iIntros "Hm".
+  iApply "HΦ".
+  rewrite map_insert_fmap.
+  iApply (is_map_retype with "Hm").
+Qed.
+
+End heap.
